equational_theories/FreeMagma.lean
@@ -27,12 +27,14 @@ def fmapFreeMagma {α : Type u} {β : Type v} (f : α → β) : FreeMagma α →
   | Lf a => FreeMagma.Leaf (f a)
   | lchild ⋆ rchild => FreeMagma.Fork (fmapFreeMagma f lchild) (fmapFreeMagma f rchild)
 
-def evalInMagma {α : Type u} {G : Type v} [Magma G] (f : α -> G) : FreeMagma α → G
+def evalInMagma {α : Type u} {G : Type v} [_root_.Magma G] (f : α -> G) : FreeMagma α → G
   | Lf a => f a
   | lchild ⋆ rchild => (evalInMagma f lchild) ∘ (evalInMagma f rchild)
 
+end FreeMagma
+
 theorem ExpressionEqualsAnything_implies_Equation2 (G: Type u) [Magma G]
-  : (∃ n : Nat, ∃ expr : FreeMagma (Fin n), ∀ x : G, ∀ sub : Fin n → G, x = evalInMagma sub expr) → Equation2 G := by
+  : (∃ n : Nat, ∃ expr : FreeMagma (Fin n), ∀ x : G, ∀ sub : Fin n → G, x = expr.evalInMagma sub) → Equation2 G := by
   intro ⟨n, expr, univ⟩ x y
   let constx : Fin n → G := fun _ ↦ x
   exact (univ x constx).trans (univ y constx).symm
@@ -52,5 +54,3 @@ theorem Equation514_implies_Equation2 (G : Type u) [Magma G]
     Lf 0 ⋆ (Lf 0 ⋆ (Lf 0 ⋆ Lf 0)), -- The syntactic representation of y ∘ (y ∘ (y ∘ y)))
     fun k sub ↦ univ k (sub 0)
   ⟩
-
-end FreeMagma
