equational_theories/MagmaLaw.lean
@@ -1,7 +1,0 @@
-import equational_theories.FreeMagma
-
-structure MagmaLaw.{u} (α : Type u) where
-  lhs : FreeMagma α
-  rhs : FreeMagma α
-
-notation:50(priority:=999) "magma law: " l " ≃ " r => MagmaLaw.mk l r
