equational_theories/Preorder.lean
@@ -1,10 +1,9 @@
 import Mathlib.Order.Defs
-import equational_theories.MagmaLaw
+import equational_theories.Completeness
 
 namespace MagmaLaw
 
-universe u
-variable {α : Type u}
+variable {α : Type}
 
 /--
 A magma law `l₁` implies a law `l₂` if in any Magma `G` where `l₁` holds, `l₂` also holds.
@@ -12,21 +11,21 @@ A magma law `l₁` implies a law `l₂` if in any Magma `G` where `l₁` holds, 
 We have to explicitly quantify the type `G` and the Magma instance `[Magma G]` instead of
 using them as parameters so that the implication holds in any Magma `G`.
 -/
-def implies (l₁ l₂ : MagmaLaw α) := ∀ {G : Type u} [Magma G] {f : α → G},
-   l₁.lhs.evalInMagma f = l₁.rhs.evalInMagma f → l₂.lhs.evalInMagma f = l₂.rhs.evalInMagma f
+def implies (l₁ l₂ : MagmaLaw α) := ∀ {G : Type} [Magma G],
+  satisfies G l₁ → satisfies G l₂
+
 
 instance : LE (MagmaLaw α) where
   le l₁ l₂ := l₁.implies l₂
 
 theorem implies_refl (l : MagmaLaw α) : l ≤ l := by
-  intro G inst f h; exact h
+  intro G inst h; exact h
 
 theorem implies_trans {l₁ l₂ l₃ : MagmaLaw α} : l₁ ≤ l₂ → l₂ ≤ l₃ → l₁ ≤ l₃ := by
-  intros h₁ h₂ G inst f h
+  intro h₁ h₂ G inst h
+  dsimp only [satisfies, satisfiesPhi] at *
   exact h₂ (h₁ h)
 
 instance : Preorder (MagmaLaw α) where
   le_refl := implies_refl
   le_trans := fun _ _ _ => implies_trans
-
-end MagmaLaw
